\documentclass{report}
\usepackage{amsmath}
\usepackage{amssymb}
\begin{document}
\section{Joint Distribution}
\subsection{Abstract}
In this section, we study Gaussian joint distribution.
\subsection{Given}
$$
x \backsim N(x|\mu, \Lambda^{-1})
$$
$$
y|x \backsim N(y|Ax+b, L^{-1})
$$
\subsubsection{Inference}
$$
y = Ax+b+\epsilon, \quad \epsilon \backsim N(0, L^{-1}), \quad x \perp \epsilon
$$
\subsection{To solve}
$$
\begin{cases}
p(y)\\
\\
p(x|y)
\end{cases}
$$
\subsection{Derivation}
\subsubsection{Derive $p(y)$}

$$
E[y] = A E[x] + b + E[\epsilon]=A \mu + b
$$
$$
Var[y] = A \Lambda^{-1} A^T
$$
$$
\therefore y \backsim N(A\mu +b, A\Lambda^{-1} A^T)
$$
\subsubsection{Derive $p(x|y)$}
\paragraph{Construct dist $z$\\}
Here we construct a distribution:
$$
z = 
\left (
\begin{matrix}
x\\
y\\
\end{matrix}
\right )
\backsim N(
\left [
\begin{matrix}
\mu\\
A\mu+b\\
\end{matrix}
\right ],
\left [
\begin{matrix}
\Lambda^{-1}&\Delta\\
\Delta&A\Lambda^{-1} A^T\\
\end{matrix}
\right ]
)
$$
$$
\begin{aligned}
\Delta
&=cov(x,y)\\
&=E[(x-E[x])(y-E[y])^T]\\
&=E[(x-\mu)(y-A\mu - b)^T]\\
&=E[(x-\mu)(Ax+b+ \epsilon -A\mu -b)^T)]\\
&=E[(x-\mu)(Ax-A\mu + \epsilon)^T]\\
&=E[(x-\mu)(x-\mu)^T A^T + (x-\mu)\epsilon^T]\\
&=E[(x-\mu)(x-\mu)^T]A^T + E[(x-\mu)\epsilon^T] \\
\because &x \perp \epsilon\\
\therefore &=E[(x-\mu)(x-\mu)^T]A^T\\
&=\Lambda^{-1}A^T
\end{aligned}
$$
$$
\therefore z=
\left ( \begin{matrix}
x\\y
\end{matrix} \right )
\backsim N(
\left [
\begin{matrix}
\mu\\
A\mu+b\\
\end{matrix}
\right ],
\left [
\begin{matrix}
\Lambda^{-1}&\Lambda^{-1}A^T\\
\Lambda^{-1}A^T&A\Lambda^{-1} A^T\\
\end{matrix}
\right ]
)
$$
\paragraph{Construct dist $x.y$\\}
let's set 
$$
\begin{aligned}
x.y 
&= x - \Sigma_{xy} \Sigma_{yy}^{-1}y\\
&= x - (\Lambda^{-1} A^T)(A \Lambda^{-1}A^T)^{-1}y\\
&= x - A^{-1}y\\
&= 
\left ( \begin{matrix}
I& -A^{-1}
\end{matrix} \right )
\left ( \begin{matrix}
x\\
y
\end{matrix} \right )
\end{aligned}
$$
$$
\begin{aligned}
E[x.y] 
&= E[x] - A^{-1} E[y]\\
&= \mu - A^{-1}(A\mu+b)\\
&= -A^{-1}b
\end{aligned}
$$
$$
\begin{aligned}
Var[x.y]
&= 
\left ( \begin{matrix}
I& -A^{-1}
\end{matrix} \right )
Var[z]
\left ( \begin{matrix}
I\\
-(A^{-1})^T\\
\end{matrix} \right )\\
&= 
\left ( \begin{matrix}
I& -A^{-1}
\end{matrix} \right )
\left (
\begin{matrix}
\Lambda^{-1}&\Lambda^{-1}A^T\\
\Lambda^{-1}A^T&A\Lambda^{-1} A^T\\
\end{matrix}
\right )
\left ( \begin{matrix}
I\\
-(A^{-1})^T\\
\end{matrix} \right )\\
&=
\left ( \begin{matrix}
\Lambda^{-1}-A^{-1} \Lambda^{-1}A^T & 0
\end{matrix} \right )
\left ( \begin{matrix}
I\\
-(A^{-1})^T\\
\end{matrix} \right )\\
&=\Lambda^{-1}-A^{-1} \Lambda^{-1}A^T
\end{aligned}
$$
$$
\therefore x.y \backsim N(-A^{-1}b, \Lambda^{-1}-A^{-1} \Lambda^{-1}A^T)
$$
\paragraph{Construct $x|y$\\}
we got
$$
x|y = x.y + A^{-1}y
$$
here, we can see $A^{-1}y$ as constant $C$.\\\\
then:
$$
x|y = x.y + C
$$
$$
E[x|y] = A^{-1}y - A^{-1}b
$$
$$
Var[x|y]= Var[x.y]
$$
$$
\therefore x|y \backsim N(A^{-1}y - A^{-1}b, \Lambda^{-1}-A^{-1} \Lambda^{-1}A^T)
$$
Now, according to an edge distribution and conditional distribution, we construct a joint distribution to obtain another edge distribution and conditional distribution.
\end{document}